Making progress

Hashmap/ForUpstream.lean
@@ -4,16 +4,6 @@
     (o.map f).isSome = o.isSome := by
   cases o <;> simp
 
-/-! From Std.Data.List.Lemmas -/
-
-@[simp] theorem List.contains_cons [BEq α] {a : α} {l : List α} {x : α} :
-    (a :: l).contains x = (x == a || l.contains x) := rfl
-
-theorem List.erase_cons [BEq α] (a b : α) (l : List α) :
-    (b :: l).erase a = if b == a then l else b :: l.erase a := by
-  cases h : b == a
-  · simp [List.erase, h]
-  · simp [List.erase, h]
 
 /-! From Std.Data.List.Basic -/
 
@@ -32,7 +22,54 @@ end
 @[simp] theorem List.pairwise_cons : Pairwise R (a::l) ↔ (∀ a' ∈ l, R a a') ∧ Pairwise R l :=
   ⟨fun | .cons h₁ h₂ => ⟨h₁, h₂⟩, fun ⟨h₁, h₂⟩ => h₂.cons h₁⟩
 
+/-- `l₁ <+ l₂`, or `Sublist l₁ l₂`, says that `l₁` is a (non-contiguous) subsequence of `l₂`. -/
+inductive List.Sublist {α} : List α → List α → Prop
+  /-- the base case: `[]` is a sublist of `[]` -/
+  | slnil : Sublist [] []
+  /-- If `l₁` is a subsequence of `l₂`, then it is also a subsequence of `a :: l₂`. -/
+  | cons a : Sublist l₁ l₂ → Sublist l₁ (a :: l₂)
+  /-- If `l₁` is a subsequence of `l₂`, then `a :: l₁` is a subsequence of `a :: l₂`. -/
+  | cons₂ a : Sublist l₁ l₂ → Sublist (a :: l₁) (a :: l₂)
+
+namespace List
+
+@[inherit_doc] scoped infixl:50 " <+ " => Sublist
+
+end List
+
+
+/-! From Std.Data.List.Lemmas -/
+
+@[simp] theorem List.contains_cons [BEq α] {a : α} {l : List α} {x : α} :
+    (a :: l).contains x = (x == a || l.contains x) := rfl
+
+theorem List.erase_cons [BEq α] (a b : α) (l : List α) :
+    (b :: l).erase a = if b == a then l else b :: l.erase a := by
+  cases h : b == a
+  · simp [List.erase, h]
+  · simp [List.erase, h]
+
+section
+
+open List
+
+theorem List.erase_sublist [BEq α] (a : α) (l : List α) : l.erase a <+ l := sorry
+
+theorem List.Pairwise.sublist (R : α → α → Prop) (l₁ l₂ : List α) : l₁ <+ l₂ → l₂.Pairwise R → l₁.Pairwise R := sorry
+
+@[simp] theorem List.Sublist.refl : ∀ l : List α, l <+ l := sorry
+
+end
+
 /-! New results -/
 
 theorem List.contains_iff_exists_beq [BEq α] (l : List α) (a : α) : l.contains a ↔ ∃ a' ∈ l, a == a' := by
   induction l <;> simp_all
+
+theorem apply_bif (f : α → β) {b : Bool} {a a' : α} :
+    f (bif b then a else a') = bif b then f a else f a' := by
+  cases b <;> simp
+
+@[simp]
+theorem bif_const {b : Bool} {a : α} : (bif b then a else a) = a := by
+  cases b <;> simp
