Hashmap/BEq.lean
@@ -29,6 +29,14 @@ theorem BEq.symm_false [BEq α] [EquivBEq α] {a b : α} : (a == b) = false → 
 theorem BEq.trans [BEq α] [EquivBEq α] {a b c : α} : a == b → b == c → a == c :=
   EquivBEq.trans
 
+theorem BEq.neq_of_neq_of_beq [BEq α] [EquivBEq α] {a b c : α} :
+    (a == b) = false → b == c → (a == c) = false := by
+  refine fun h₁ h₂ => Bool.eq_false_iff.2 fun h₃ => Bool.eq_false_iff.1 h₁ (BEq.trans h₃ (BEq.symm h₂))
+
+theorem BEq.neq_of_beq_of_neq [BEq α] [EquivBEq α] {a b c : α} :
+    a == b → (b == c) = false → (a == c) = false := by
+  refine fun h₁ h₂ => Bool.eq_false_iff.2 fun h₃ => Bool.eq_false_iff.1 h₂ (BEq.trans (BEq.symm h₁) h₃)
+
 instance (priority := low) [BEq α] [LawfulBEq α] : EquivBEq α where
   refl := LawfulBEq.rfl
   symm h := (beq_iff_eq _ _).2 <| Eq.symm <| (beq_iff_eq _ _).1 h
